Examples/arm7_collatz_smc.v
@@ -1,0 +1,73 @@
+Require Import NArith.
+Require Import ZArith.
+Require Import Picinae_armv7_lifter.
+Require Import List.
+Require Import String.
+Import ListNotations.
+Open Scope Z.
+
+Definition rz   := 0.
+Definition r    := 1.
+Definition r'   := 2.
+Definition tr   := 5.
+Definition rout := 0.
+Definition pc   := 15.
+Definition LR   := 14.
+Definition always := 14. (* Uncondtional cond code *)
+Definition left := 0.
+Definition right := 2.
+
+(* Receive input inp in register 0, named rz and used to store 0 in the code.
+   Move inp from rz to r, load 0 into rz.
+   Evaluate tr to be the code for rz if inp is even, code for r if it is odd.
+   Update the final ADD instruction to add the register referred to by tr. 
+
+   NB: The first PIL statement to execute in each instruction loads the PC
+       into R_PC.
+
+  Equivalent assembly:
+
+    _start:
+256     mov r1, r0
+260     mov r0, #0
+264     eor r5, r1, #1
+268     strb r5, [pc, #11] ---+ Overwrite the r8 operand byte.
+                              | It becomes either r or rz.
+272     add r2, r1, #1        | The other bits in this byte
+276     lsr r2, r2, #1        | are conveniently all zeros.
+280     add r0, r2, r8   <----+
+284     bx lr 
+
+  *)
+
+(*Compute arm_decode 0xe0820008.
+Compute arm_decode 8519688.
+Compute arm_decode 0x00820008.*)
+Definition collatz_prog :=  [
+  (* ARM_data_i (op: arm_data_op) (cond S Rn Rd imm12: Z) *)
+  (* 0: *) ARM_data_i ARM_ADD always 0 rz r  0x0;
+  (* 1: *) ARM_data_i ARM_MOV always 0 0  rz 0x0;
+  (* 2: *) ARM_data_i ARM_AND always 0 r  tr 0x1;
+  (* ARM_ls_i (op: arm_mem_op) (cond P U W Rn Rt imm12: Z) *)
+  (* 3: *) ARM_ls_i ARM_STRB always 1 1 0 pc tr (4*1); (* Overwrite the last byte in instruction #6 *)
+  (* Update Operands *)
+  (* ARM_data_i (op: arm_data_op) (cond S Rn Rd imm12: Z) *)
+  (* 4: *) ARM_data_i ARM_ADD always 0 r r' 0x1;
+  (* ARM_data_r (op: arm_data_op) (cond S Rn Rd imm5 type Rm: Z) *)
+  (* 5: *) ARM_data_r ARM_MOV always 0 0 r' 0x1 1 r';
+  (* 6: *) ARM_data_r ARM_ADD 14 0 r' rout 0 0 0x8; (* The 0x8 gets overwritten at runtime *)
+  (* End of update *)
+  (* 7: *) ARM_BX always LR
+  ].
+
+
+Open Scope N.
+Compute arm_assemble_all collatz_prog.
+Compute print_code_prop 32 LittleE "V_MEM32" collatz_prog 0x100 "collatz_arm7".
+Compute print_exec_prop collatz_prog 0x100 "collatz_arm7".
+
+Definition collatz_arm7 (s:store) : Prop :=
+ getmem 32 LittleE 32 (s V_MEM32) 256 = 
+        101855193521039785343392224741083126283860177008767390847333957731433903558656.
+Definition collatz_arm7_aexec (mem:N) : Prop :=
+  xbits mem 256 288 = 4294967295.
