Examples/arm7_collatz_smc_proof.v
@@ -1,0 +1,111 @@
+Require Import Picinae_theory.
+Require Import arm7_collatz_smc.
+Require Import Picinae_armv7.
+Require Import -(notations) Picinae_armv7_lifter.
+Require Import NArith.
+Require Import Lia ZifyN ZifyBool.
+Open Scope N.
+
+Import ARM7Notations.
+
+Definition collatz_start : N :=  0x100.
+Definition collatz_end   : N :=  0x100 + 4 * 7.
+
+Section Invariants.
+  Variables inp : N.
+  Variable  s0 : store.
+
+  Definition postcondition (s:store) :=
+    s R_R0 = if N.even inp then inp >> 1 else inp ⊕ (1 ⊕ inp >> 1).
+  Definition mem_unchanged (s:store) := s V_MEM32 = s0 V_MEM32.
+  Definition invs (t:trace) : option Prop:=
+    match t with (Addr a, s) :: _ => match a with
+      | 0x100 => Some (mem_unchanged s /\ s R_R0 = inp /\ s R_T = 0 /\ s R_JF = 0 /\ s R_E = 0)
+      | 0x11c => Some (postcondition s)
+      | _ => None end
+    | _ => None end.
+End Invariants.
+
+Definition collatz_exit (t:trace) :=
+  match t with (Addr a,_)::_ => match a with
+  | 0x11c => true
+  | _ => false
+  end | _ => false end.
+
+Theorem collatz_correctness:
+  forall s t s' x' inp
+         (ENTRY: startof t (x',s') = (Addr 0x100,s))
+         (MDL: models arm7typctx s)
+         (RT: s R_T = 0)
+         (JF: s R_JF = 0)
+         (RE: s R_E = 0)
+         (INP: s R_R0 = inp)
+         (MEM: collatz_arm7 s)
+,
+(* We define our program as p32_prog, a function that looks into
+   a given store's memory and page-execute permissions to determine
+   what the next instruction is.
+   Above we specified that the memory of the initial store is exactly
+   our program, which is held in bytes 0-12 with all other bytes 0.
+*)
+  satisfies_all arm_prog (invs inp s) collatz_exit ((x',s')::t).
+Proof.
+Local Ltac step := time ISA_step.
+intros. unfold satisfies_all.
+  apply prove_invs.
+  (* Base case: *)
+  simpl. rewrite ENTRY.
+  step. repeat (split; try assumption).
+
+  (* Inductive cases *)
+  intros.
+  (* somehow `startof_prefix` is bound to the wrong theorem here...
+     In the strspn example the theorem is preferentially bound to
+     Picinae.Picinae_armv8.Theory_arm8.startof_prefix
+     rather than the alternative Picinae.Picinae_theory.startof_prefix.
+     Here it is the opposite, so we must specify the arch-specific version*)
+  erewrite startof_prefix in ENTRY; try eassumption.
+  eapply models_at_invariant; try (eassumption || apply welltyped_arm_prog).
+  clear MDL; intros MDL.
+  clear - PRE MDL MEM. rename s into s0, t1 into t, s1 into s.
+
+  destruct_inv 32 PRE.
+  destruct PRE as (MEMSAME & INP & RT & JF & RE).
+  unfold collatz_arm7 in MEM.
+  rewrite <-MEMSAME in *. clear MEMSAME.
+  step.
+  step.
+  step.
+  step.
+  step.
+  step.
+
+  assert (inp mod 2 < 2) by lia.
+  destruct (inp mod 2) as [|p] eqn:EQ; try destruct p; try lia.
+
+  step.
+  assert (H0:N.even inp = true).
+  rewrite <-testbit0_even, Bool.negb_true_iff, N.bit0_eqb, EQ. easy. rewrite H0.
+  apply N.bits_inj; intro.
+  rewrite !N.shiftr_spec; try lia.
+  assert (forall w a b, a mod 2^w = 0 -> b < 2^w -> forall i, i >= w -> N.testbit a i = N.testbit (a+b) i).
+  clear - s0. induction w using N.peano_ind; clear s0; intros.
+    destruct b; try lia. rewrite N.add_0_r; reflexivity.
+    rewrite mp2_mod_divides in H. destruct H as [m EQ].
+    destruct (N.zero_or_succ i); try lia. destruct H as [i' Eq]; subst i.
+    assert (H2: i' >= w) by lia; clear H1.
+    Search (N.testbit _ (N.succ _)). rewrite <-!N.div2_bits.
+    assert (H:(a+b)/2 = a/2 + b/2) by admit. (* maybe use mp2_div_add here *)
+    rewrite H.
+    apply IHw; try lia. admit. admit.
+  specialize (H1 1 inp 1). psimpl in H1. assert (HELP: n+1>=1) by lia.
+  specialize (H1 EQ (eq_refl _) (n+1) HELP); clear HELP.
+  rewrite H1.
+  Unset Printing Notations.
+  admit.
+
+  step.
+  assert (H0: N.even inp = false).
+  rewrite <-testbit0_even, Bool.negb_false_iff, N.bit0_eqb, EQ. easy. rewrite H0.
+  lia.
+Time Qed.
