Picinae_SMC.v
@@ -1,0 +1,286 @@
+(* Picinae: Platform In Coq for INstruction Analysis of Executables       ZZM7DZ
+                                                                          $MNDM7
+   Copyright (c) 2025 Kevin W. Hamlen            ,,A??=P                 OMMNMZ+
+   The University of Texas at Dallas         =:$ZZ$+ZZI                  7MMZMZ7
+   Computer Science Department             Z$$ZM++O++                    7MMZZN+
+                                          ZZ$7Z.ZM~?                     7MZDNO$
+                                        ?Z8ZO7.OM=+?                     $OMO+Z+
+   Any use, commercial or otherwise       ?D=++M++ZMMNDNDZZ$$Z?           MM,IZ=
+   requires the express permission of        MZZZZZZ+...=.8NOZ8NZ$7       MM+$7M
+   the author.                                 ?NNMMM+.IZDMMMMZMD8O77     O7+MZ+
+                                                     MMM8MMMMMMMMMMM77   +MMMMZZ
+                                                     MMMMMMMMMMMZMDMD77$.ZMZMM78
+                                                      MMMMMMMMMMMMMMMMMMMZOMMM+Z
+   Support code for instantiating Picinae to           MMMMMMMMMMMMMMMMM^NZMMN+Z
+   various particular Instruction Set Architectures.    MMMMMMMMMMMMMMM/.$MZM8O+
+                                                         MMMMMMMMMMMMMM7..$MNDM+
+   To compile this module, first load and compile:        MMDMMMMMMMMMZ7..$DM$77
+   * Picinae_core                                          MMMMMMM+MMMZ7..7ZM~++
+                                                            MMMMMMMMMMM7..ZNOOMZ
+                                                             MMMMMMMMMM$.$MOMO=7
+                                                              MDMMMMMMMO.7MDM7M+
+   Then compile this module with menu option                   ZMMMMMMMM.$MM8$MN
+   Compile->Compile_buffer.                                    $ZMMMMMMZ..MMMOMZ
+                                                                ?MMMMMM7..MNN7$M
+                                                                 ?MMMMMZ..MZM$ZZ
+                                                                  ?$MMMZ7.ZZM7DZ
+                                                                    7MMM$.7MDOD7
+                                                                     7MMM.7M77ZZ
+                                                                      $MM78ZDZ7Z
+                                                                        MM8D$7Z7
+                                                                        MM7O$$+Z
+                                                                         M 7N8ZD
+ *)
+
+Require Import Picinae_core.
+Require Import Picinae_theory.
+Require Import Picinae_statics.
+Require Import Picinae_finterp.
+Require Import Picinae_simplifier_base.
+Require Import NArith.
+Require Import Program.Equality.
+Require Import Structures.Equalities.
+Require Import Picinae_ISA.
+Open Scope N.
+
+Module Type PICINAE_SMC.
+  Parameter asm : Set.
+  Parameter insn_length : asm -> N.
+  Parameter assemble_insn : asm -> N.
+End PICINAE_SMC.
+
+Require Import String.
+Require Import Ascii.
+Require Import Recdef.
+Require Import Program.
+Require Import Lia.
+
+Open Scope string.
+Open Scope N.
+
+Module Picinae_SMC (IL: PICINAE_IL)  (PSIMPL:PSIMPL_BASE IL)
+  (TIL: PICINAE_THEORY IL)
+  (SIL: PICINAE_STATICS IL TIL)
+  (FIL: PICINAE_FINTERP IL TIL SIL)
+  (SMC: PICINAE_SMC).
+Module ISA := Picinae_ISA IL PSIMPL TIL SIL FIL.
+
+Import IL.
+Import SMC.
+Import PSIMPL.
+Import TIL.
+Export ISA.
+
+Definition code_length (code:list asm) : N :=
+  List.fold_left N.add (List.map insn_length code) 0%N.
+
+(* Will we ever need to pass the instruction address to the assemble_insn function? *)
+Fixpoint assemble' (b mem:N) (code:list asm) : N :=
+  match code with
+  | nil => mem
+  | insn :: t => assemble' (b+insn_length insn) (setmem 32 LittleE (insn_length insn) mem b (assemble_insn insn)) t
+  end.
+
+Definition assemble b code := assemble' b 0%N code.
+
+Definition newline :string := String "010" EmptyString.
+
+Program Fixpoint N2str_impl (n:N) (acc:string) {measure (N.to_nat n)}: string :=
+  (match n with
+    | 0%N => String "0" acc
+    | 1%N => String "1" acc
+    | 2%N => String "2" acc
+    | 3%N => String "3" acc
+    | 4%N => String "4" acc
+    | 5%N => String "5" acc
+    | 6%N => String "6" acc
+    | 7%N => String "7" acc
+    | 8%N => String "8" acc
+    | 9%N => String "9" acc
+    | _ => N2str_impl (n/10)
+       (String (match (n mod 10)%N with
+         | 0%N => "0"
+         | 1%N => "1"
+         | 2%N => "2"
+         | 3%N => "3"
+         | 4%N => "4"
+         | 5%N => "5"
+         | 6%N => "6"
+         | 7%N => "7"
+         | 8%N => "8"
+         | 9%N => "9"
+         | _ => "!"
+       end) acc)
+  end)%nat .
+Next Obligation. lia. Defined.
+Next Obligation. lia. Defined.
+Next Obligation. lia. Defined.
+Next Obligation. lia. Defined.
+Next Obligation. lia. Defined.
+Next Obligation. lia. Defined.
+Next Obligation. lia. Defined.
+Next Obligation. lia. Defined.
+Next Obligation. lia. Defined.
+Next Obligation. lia. Defined.
+Next Obligation. lia. Defined.
+Next Obligation. lia. Defined.
+Next Obligation. lia. Defined.
+Next Obligation. lia. Defined.
+Next Obligation. lia. Defined.
+Next Obligation. lia. Defined.
+Next Obligation. lia. Defined.
+Next Obligation. lia. Defined.
+Next Obligation. lia. Defined.
+Next Obligation. lia. Defined.
+Next Obligation. lia. Defined.
+
+Definition N2str n := N2str_impl n "".
+
+(* All ways of converting numbers to Rocq strings require using "to_nat" which blows up
+   the computation process, severely limiting the magnitude of numbers Rocq can convert
+   to strings within its TCB.  Thus `Compute N2str assemble base code.` freezes until it
+   runs out of memory or the user gets bored. Either way we cannot pring a string containing
+   the numeric expression of the code, so we compute the expression and return it as an
+   element in the tuple for Rocq's to convert to a string outside of the trusted kernel. *)
+Definition endian2str e :=
+  match e with
+  | LittleE => "LittleE"
+  | BigE => "BigE"
+  end.
+
+Definition print_code_prop (w:bitwidth) e (vmem:string) (code:list asm) (base_addr:N) (name:string) :=
+  ("Definition " ++ name ++ " (s:store) : Prop :=" ++ newline ++
+    " getmem " ++ (N2str w) ++ " " ++ (endian2str e) ++ " " ++
+    (N2str ((code_length code))) ++ " (s " ++ vmem ++ ") " ++ (N2str base_addr) ++ " = " ++
+  "XXXX" ++ ".",
+  (assemble 0 code)).
+
+(* We use an xbits implementation instead of getmem because each bit corresponds to a byte,
+   using getmem means we cannot set individual bytes to be executable/not executable, our
+   finest granularity with getmem/setmem would be 8 bytes at a time.  Do we need byte-level
+   granularity?  Unsure. *)
+Definition print_exec_prop (code:list asm) (base_addr:N) (name:string) :=
+  ("Definition " ++ name ++ "_aexec (mem:N) : Prop :=" ++ newline ++
+  "  xbits mem " ++ (N2str base_addr) ++ " " ++
+  (N2str (base_addr + (code_length code))) ++ " = " ++
+  "XXXX" ++ "." ++ newline
+  , N.ones (code_length code) ).
+
+Ltac unfold_store_props :=
+  repeat match goal with
+  | [P: ?prop (?s _) |- _ ] => match type of s with store => unfold prop in P end
+  end.
+
+(* Does not yet support permission bit modification. No code we have modeled updates
+   permission bits, so we have not needed it. But we can extend it the same way we
+   can model updates to the code. *)
+Ltac get_exec :=
+  repeat match goal with
+  (* Frame out store updates from the exec permission read *)
+  | [H: xbits (_ ?m) _ _ = _ |- context[N.testbit (update ?s _ _ ?m) _]] =>
+    rewrite (update_frame s _ _ m);[|easy]
+  (* Finally, now that we are reading the bit from the same variable (e.g., `s A_EXEC`) that
+     we have a proposition about we can evaluate what the bit is.  The `assert HELP` ensures
+     we are using the right proposition by checking the bit we are reading is within the bounds.
+     We use an assert instead of failure because we want to use `try lia` to address the arithmetic
+     goals instead of the more syntactically cumbersome and fragile goal selectors. *)
+  | [H: xbits ?v ?l ?h = ?mem |- context[N.testbit ?v ?i]] =>
+    let HELP := fresh "H" in
+    assert (HELP: l <= i /\ i <= h) by (split; lia); clear HELP;
+    rewrite testbit_xbits, (xbits_split2 l i (N.succ i) h v mem);
+    try lia; vm_compute (N.odd _)
+  end.
+
+Ltac unfold_prog_hook := idtac "You need to override this Ltac with an ltac unfolding the definition(s) of your memory-decoding program function.";
+  idtac "E.g., `Ltac unfold_prog_hook ::= unfold p32_prog, p32_stmt."; fail.
+
+Ltac reduce_frames :=
+  repeat match goal with
+         | |- context[update ?s _ _ ?m] => rewrite (update_frame s _ _ m);[|easy]
+         end.
+
+Ltac rewrite_vars :=
+  repeat match goal with
+  | [S: store, H: ?S ?v = _ |- context[?S ?v]] => rewrite H in *
+  end.
+
+Ltac reduce_getmem_hyp :=
+  match goal with
+  | MEM: getmem _ _ _ ?m _ = _ |- context[getbyte ?m _ _] =>
+      erewrite (getmem_byte MEM); try lia; first [timeout 1 vm_compute xbits | idtac]
+  end.
+
+(* Solves simple existentially quantified sums. E.g., `4 = 1 + ?i`. *)
+Ltac solve_sum :=
+  match goal with |- ?n = 1 + _ => replace n with (1+(n-1)) by lia; simpl N.sub; reflexivity end.
+
+Ltac reduce_getmem x H :=
+  let htyp := type of H in
+  lazymatch ltac:(constr:((htyp,x))) with
+  | (getmem _ _ _ _ _ = _, getmem _ _ _ _ _) =>
+    let H := fresh "H" in
+    eassert (H: x = _);[
+        reduce_frames;
+        try rewrite update_updated;
+        repeat (erewrite getmem_first;[
+          (* Make progress removing non-overlapping memory writes,
+             or if it does overlap then interpret the byte from it. *)
+          repeat match goal with
+                | |- context[getbyte (setmem ?w _ ?len _ ?a ?v) ?b ?w] =>
+                    first [
+                      rewrite getbyte_noverlap;[|apply noverlap_sum; timeout 1 vm_compute msub; lia]
+                    | let i := constr:(b - a) in
+                        replace b with (a + i) by lia;
+                        rewrite setmem_byte;[|lia|lia]
+                    ]
+                end;
+          try reduce_getmem_hyp
+
+      | solve_sum ]);
+      rewrite getmem_0;
+      (*  At this point the goal is `byte_1 .| byte_2 .| ... .| 0 = ?Goal`
+          We need to use psimpl on the left hand side only, otherwise it
+          instantiates the evar ?Goal to 0. *)
+      match goal with |- ?lhs = _ => psimpl lhs end; reflexivity
+  |];
+(* Do not put the `rewrite H` inside of the [|] tactical to force evar instantiation before use. *)
+  rewrite H in *; clear H
+  | _ => idtac "Input was not a getmem call."; fail
+  end.
+
+Ltac reduce_testbitmem x H :=
+  let htyp := type of H in
+  lazymatch ltac:(constr:((htyp, x))) with
+  | (xbits ?b ?l ?h = ?mem, N.testbit ?v ?i) => 
+    let HELP := fresh "H" in
+    assert (HELP: l <= i /\ i <= h) by (split; lia); clear HELP;
+    rewrite testbit_xbits, (xbits_split2 l i (N.succ i) h v mem);
+    try lia; vm_compute (N.odd _)
+  end.
+
+(* These hooks are used in ISA_invseek to simplify the memory program
+   instruction expression which, for an interpreted language like this
+   one, is read as bytes from memory then decoded. *)
+Global Ltac effinv_none_hook ::=
+  unfold effinv, effinv';
+  unfold_prog_hook;
+  unfold_store_props;
+  reduce_frames;
+  rewrite_vars;
+  repeat match goal with
+         | H: xbits ?v _ _ = _ |- context[N.testbit ?v ?m] => reduce_testbitmem (N.testbit v m) H
+         end;
+  repeat  match goal with
+          | MEM: getmem _ _ _ _ _ = _ |- context[getmem ?w ?e ?len ?m ?a] => idtac len m a;
+              reduce_getmem (getmem w e len m a) MEM
+          end;
+  first [timeout 2 vm_compute | idtac].
+
+(* Original version had a different ltac for decoding instructions, but the arm7 architecture
+   shows that some architectures require decoding instructions to tell if the program effectively
+   exited. So now effinv_none_hook includes the decoding machinery as well and `psa_some_hook`
+   is redundant by default but available for fine tuning the machinery. *)
+Ltac psa_some_hook ::= 
+  effinv_none_hook.
+
+End Picinae_SMC.
